saketh's solution for whiteblackball

WeeklyLean/WhiteBlackBall/saketh.lean
@@ -1,81 +1,196 @@
 structure Bag where
-  numBlackBalls: Int
-  numWhiteBalls: Int
-
-inductive Turn where
-| ww_w
-| wb_b
-| bb_w
+  numBlackBalls: Nat
+  numWhiteBalls: Nat
+deriving Repr
 
 inductive Step : Bag → Bag → Prop where
-| ww_w (w: Int) (b: Int) : w >= 2 →
+| ww_w (w: Nat) (b: Nat) : w >= 2 →
          b >= 0 →
          Step
           {numBlackBalls := b, numWhiteBalls := w}
           {numBlackBalls := b, numWhiteBalls := w - 1}
-| wb_b (w: Int) (b: Int) : w >= 1 →
+| wb_b (w: Nat) (b: Nat) : w >= 1 →
          b >= 1 →
           Step
           {numBlackBalls := b, numWhiteBalls := w}
           {numBlackBalls := b , numWhiteBalls := w - 1}
-| bb_w (w: Int) (b: Int) : w >= 0 →
+| bb_w (w: Nat) (b: Nat) : w >= 0 →
          b >= 2 →
           Step
           {numBlackBalls := b, numWhiteBalls := w}
           {numBlackBalls := b - 2, numWhiteBalls := w + 1}
 
 inductive StepStar: Bag → Bag → Prop where
-| ending : s.numBlackBalls >= 0
-  -> s.numWhiteBalls >= 0
-  -> s.numBlackBalls + s.numWhiteBalls = 1
-  -> StepStar s s
+| refl : StepStar s s
 | step : Step s1 s2 → StepStar s2 s3 → StepStar s1 s3
 
+def numBalls (b: Bag) : Nat :=
+  b.numBlackBalls + b.numWhiteBalls
 
-theorem sizeDecreases (h: Step s1 s2) :
-  s2.numBlackBalls + s2.numWhiteBalls
-  = s1.numBlackBalls + s1.numWhiteBalls - 1 := by
-  cases h
-  case ww_w =>
-    simp [Bag.numBlackBalls, Bag.numWhiteBalls]
-    omega
-  case wb_b =>
-    simp [Bag.numBlackBalls, Bag.numWhiteBalls]
-    omega
-  case bb_w =>
-    simp [Bag.numBlackBalls, Bag.numWhiteBalls]
+def isFinalState (s: Bag) : Prop :=
+  s.numBlackBalls + s.numWhiteBalls = 1
+
+def isValid (b: Bag) : Prop :=
+  numBalls b > 0
+
+theorem sizeDecreases :
+  ∀ s1: Bag, ∀ s2: Bag,
+  numBalls s1 > 1 ->
+  Step s1 s2 ->
+  numBalls s2 = (numBalls s1) - 1 := by
+    intros s1 s2 Hsize Hstep
+    cases Hstep with
+    | ww_w w b Hw Hb => simp [numBalls]
+                        omega
+    | wb_b w b Hw Hb => simp [numBalls]
+                        omega
+    | bb_w w b Hw Hb => simp [numBalls]
+                        omega
+
+theorem finalStateCannotStep (finalState: Bag) :
+  isFinalState finalState -> ¬ exists s : Bag, Step finalState s := by
+    intros Hfinal Hexists
+    cases Hexists with
+    | intro s Hstep => cases Hstep with
+      | ww_w w b Hw Hb => simp [isFinalState] at Hfinal
+                          omega
+      | wb_b w b Hw Hb => simp [isFinalState] at Hfinal
+                          omega
+      | bb_w w b Hw Hb => simp [isFinalState] at Hfinal
+                          omega
+
+theorem progress (state: Bag) :
+  isValid state →
+  ¬ isFinalState state ->
+    ∃ s : Bag, Step state s := by
+  intros Hvalid HnonFinal
+  simp [isValid, numBalls] at Hvalid
+  simp [isFinalState] at HnonFinal
+  have HmoreThanOneBall: state.numBlackBalls + state.numWhiteBalls > 1 := by
+    simp [numBalls]
     omega
 
+  have Hcondition: state.numWhiteBalls >= 2 ∨ ¬ state.numWhiteBalls >= 2 := by
+    apply Decidable.em
+  cases Hcondition with
+  -- numWhiteBalls >= 2
+  | inl Hw =>
+    exists {numBlackBalls := state.numBlackBalls, numWhiteBalls := state.numWhiteBalls - 1}
+    apply Step.ww_w <;> omega
+  -- numWhiteBalls < 2
+  | inr Hw =>
+  have Hcondition': state.numBlackBalls >= 2 ∨ ¬ state.numBlackBalls >= 2 := by
+    apply Decidable.em
+  cases Hcondition' with
+  -- numBlackBalls >= 2
+  | inl Hb =>
+    exists {numBlackBalls := state.numBlackBalls - 2, numWhiteBalls := state.numWhiteBalls + 1}
+    apply Step.bb_w <;> omega
+  -- numBlackBalls < 2
+  | inr Hb =>
+    exists {numBlackBalls := state.numBlackBalls, numWhiteBalls := state.numWhiteBalls - 1}
+    apply Step.wb_b <;> omega
+
+
+
+-- induction on size
+-- if size is 0, then it's a contradiction as we can't have a bag with 0 balls
+-- if size is 1, then it must be final
+-- if size is greater than 1, then we can apply one step rule
+theorem terminates :
+  ∀ nb: Nat, ∀ start: Bag,
+  numBalls start = nb →
+  isValid start →
+  ∃ finish: Bag, ∃ stepStar: StepStar start finish,
+    isFinalState finish := by
+    intro numBalls
+    cases numBalls
+    -- numBalls = 0: contradiction
+    case zero => intros start HnumBalls Hvalid; simp [isValid, numBalls] at *; omega
+    case succ n =>
+    induction n
+    -- numBalls = 1: final state, finish = start
+    case zero =>
+      simp [isFinalState]
+      intros start HnumBalls Hvalid
+      simp [isValid, numBalls] at *
+      exists start
+      constructor
+      . constructor
+      . omega
+    -- numBalls > 1: apply one step then induct
+    case succ n' IH =>
+    simp [isFinalState]
+    simp at IH
+    intros start HnumBalls Hvalid
+    simp [isValid, numBalls] at *
+    have HnonFinal: ¬ isFinalState start := by
+      intro Hfinal
+      simp [isFinalState] at Hfinal
+      omega
+
+    -- there exists a state s that can be reached from start
+    have HstepExists: ∃ s : Bag, Step start s := by
+      apply progress
+      . simp [isValid, numBalls]; omega
+      . assumption
+
+    have HmoreThanOneBall: numBalls start > 1 := by
+      simp [numBalls]
+      omega
+
+
+    cases HstepExists; case intro s Hstep =>
+    -- build a step star using Hstep.
+    -- start -Hstep-> s -Hstepstar-> finish
+    -- since for every s, there exists a finish, we can use this to build a finish
+    have H1 : numBalls s = numBalls start - 1 := by
+      apply sizeDecreases start s HmoreThanOneBall Hstep
+
+    simp [numBalls] at H1
+    have HsSize: n' + 1 = s.numBlackBalls + s.numWhiteBalls := by omega
+
+    have HfinishExists: ∃ finish: Bag, StepStar s finish ∧ isFinalState finish
+      := by apply IH s <;> omega
+
+    cases HfinishExists with
+    | intro finish' Hfinish' =>
+
+    simp [isFinalState] at Hfinish'
+    cases Hfinish' with
+    | intro Hstepstar Hfinal =>
+
+    exists finish'
+    constructor
+    . apply StepStar.step Hstep Hstepstar
+    . assumption
 
 theorem evenBlackStepsToWhite (start: Bag) (ending: Bag) :
   start.numBlackBalls % 2 = 0 →
   StepStar start ending →
+  isFinalState ending ->
   ending.numBlackBalls = 0 && ending.numWhiteBalls = 1 := by
-    intros Heven Hstepstar
+    intros Heven Hstepstar Hfinal
     simp [Bag.numBlackBalls, Bag.numWhiteBalls]
     induction Hstepstar
-    case ending => omega
+    case refl next => simp [isFinalState] at Hfinal; omega
     case step s1 s2 s3 S SS IH =>
       have H: s2.numBlackBalls % 2 = 0 := by cases S with
         | ww_w w b Hw Hb  => apply Heven
         | wb_b w b Hw Hb  => apply Heven
-        | bb_w w b Hw Hb  => simp [Bag.numBlackBalls] at Heven
-                            simp [Bag.numBlackBalls]
-                            assumption
-      apply IH
-      apply H
-
-
-
+        | bb_w w b Hw Hb  => simp [Bag.numBlackBalls] at *; omega
+      apply IH H Hfinal
 
 theorem oddBlackStepsToBlack (start: Bag) :
   start.numBlackBalls % 2 = 1 →
   StepStar start ending ->
+  isFinalState ending ->
   ending.numBlackBalls = 1 && ending.numWhiteBalls = 0 := by
-    intros Hodd Hstepstar
+    intros Hodd Hstepstar Hfinal
     simp [Bag.numBlackBalls, Bag.numWhiteBalls]
+    simp [isFinalState] at Hfinal
     induction Hstepstar
-    case ending => omega
+    case refl => omega
     case step s1 s2 s3 S SS IH =>
       have H: s2.numBlackBalls % 2 = 1 := by cases S with
         | ww_w w b Hw Hb  => simp [Bag.numBlackBalls] at Hodd
@@ -86,6 +201,5 @@ theorem oddBlackStepsToBlack (start: Bag) :
                              assumption
         | bb_w w b Hw Hb  => simp [Bag.numBlackBalls] at Hodd
                              simp [Bag.numBlackBalls]
-                             assumption
-      apply IH
-      apply H
+                             omega
+      apply IH H Hfinal
